TM/Code/MatchFin.v
@@ -17,12 +17,12 @@ Section MatchFin.
     Move R tt;;
     MATCH (Read_char)
     (fun s => match s with
-           | Some (inr x) => Move L x
+           | Some (inr x) => Move R x
            | _ => mono_Nop default
            end).
 
   Definition MatchFin_Rel : pRel sig^+ sig 1 :=
-    fun tin '(yout, tout) => forall x : sig, tin[@Fin0] ≃ x -> tout[@Fin0]≃x /\ yout = x.
+    fun tin '(yout, tout) => forall x : sig, tin[@Fin0] ≃ x -> isRight tout[@Fin0] /\ yout = x.
 
   Lemma MatchFin_Sem : MatchFin ⊨c(5) MatchFin_Rel.
   Proof.
@@ -44,3 +44,14 @@ End MatchFin.
 
 Arguments MatchFin : simpl never.
 Arguments MatchFin sig {_}. (* Default element is infered automatically *)
+
+
+
+Ltac smpl_TM_MatchFin :=
+  match goal with
+  | [ |- MatchFin _ ⊨ _ ] => eapply RealiseIn_Realise; apply MatchFin_Sem
+  | [ |- MatchFin _ ⊨c(_) _ ] => apply MatchFin_Sem
+  | [ |- projT1 (MatchFin _) ↓ _ ] => eapply RealiseIn_terminatesIn; apply MatchFin_Sem
+  end.
+
+Smpl Add smpl_TM_MatchFin : TM_Correct.
